Checkpoint

code/mlkem/Hacl.MLkem.Poly.fst
@@ -59,15 +59,17 @@ val add:
     disjoint a b /\
     disjoint a res /\
     disjoint b res /\
-    modifies (loc res) h0 h1
-    // Seq.equal (lpoly_v h1 res) (S.add (lpoly_v h1 a) (lpoly_v h1 b))
+    modifies (loc res) h0 h1 /\
+    Seq.equal (lpoly_v h1 res) (S.add (lpoly_v h0 a) (lpoly_v h0 b))
    )
 
 let add #deg a b res =
   push_frame ();
   let h0 = ST.get () in
   let inv h (i:nat) =
-    live h a /\ live h b /\ live h res /\ modifies (loc res) h0 h in
+    live h a /\ live h b /\ live h res /\ modifies (loc res) h0 h /\
+    i <= v deg /\
+    Seq.equal (Seq.slice (lpoly_v h res) 0 i) (Seq.slice (S.add (lpoly_v h a) (lpoly_v h b)) 0 i) in
   let body (i: U32.t{ 0 <= U32.v i /\ U32.v i < U32.v deg }):
     Stack unit
     (requires (fun h -> inv h (U32.v i)))
@@ -75,6 +77,9 @@ let add #deg a b res =
     = let ai = a.(i) in
       let bi = b.(i) in
       let sum = add_zq ai bi in
-      res.(i) <- sum in
+      res.(i) <- sum;
+      let hx = ST.get () in
+      assume (inv hx (U32.v i + 1))
+    in
   Lib.Loops.for 0ul deg inv body;
   pop_frame ()
